feat(Computability): improve structure, refactor
move `time` def to Complexity
move `computes` def to Computability

Complexity.thy
@@ -6,15 +6,152 @@ theory Complexity
   imports TM_Hoare Goedel_Numbering
 begin
 
-subsubsection\<open>Time\<close>
+subsection\<open>Time\<close>
 
 text\<open>The time restriction predicate is similar to \<^term>\<open>Hoare_halt\<close>,
   but includes a maximum number of steps.
   From @{cite \<open>ch.~12.1\<close> hopcroftAutomata1979}:
   ``If for every input word of length n, M makes at most T(n) moves before
     halting, then M is said to be a T(n) time-bounded Turing machine, or of time
-    complexity T(n). The language recognized by M is said to be of time complexity T(n).''
+    complexity T(n). The language recognized by M is said to be of time complexity T(n).''\<close>
 
+context TM
+begin
+
+definition "config_time c \<equiv> LEAST n. is_final (steps n c)"
+
+lemma steps_conf_time[intro, simp]:
+  assumes "is_final (steps n c)"
+  shows "steps (config_time c) c = steps n c"
+proof -
+  from assms have "is_final (steps (config_time c) c)" unfolding config_time_def by (rule LeastI)
+  then show ?thesis using assms by (rule final_steps_rev)
+qed
+
+lemma conf_time_lessD[dest, elim]: "n < config_time c \<Longrightarrow> \<not> is_final (steps n c)"
+  unfolding config_time_def by (rule not_less_Least)
+
+lemma conf_time_geD[dest, elim]:
+  assumes "n \<ge> config_time c"
+    and "halts_config c"
+  shows "is_final (steps n c)"
+proof -
+  from assms(2) have "is_final (steps (LEAST n. is_final (steps n c)) c)"
+    unfolding halts_config_def by (rule LeastI_ex)
+  with assms(1) show ?thesis unfolding config_time_def by blast
+qed
+
+lemma conf_time_geI[intro]: "is_final (steps n c) \<Longrightarrow> config_time c \<le> n"
+  unfolding config_time_def run_def by (fact Least_le)
+
+lemma conf_time_ge_iff[intro]: "halts_config c \<Longrightarrow> is_final (steps n c) \<longleftrightarrow> n \<ge> config_time c"
+  by blast
+
+lemma conf_time_less_rev[intro]: "halts_config c \<Longrightarrow> \<not> is_final (steps n c) \<Longrightarrow> n < config_time c"
+  by (subst (asm) conf_time_ge_iff) auto
+
+lemma conf_time_finalI[intro]: "halts_config c \<Longrightarrow> is_final (steps (config_time c) c)"
+  using conf_time_ge_iff by blast
+
+lemma conf_time0[simp, intro]: "is_final c \<Longrightarrow> config_time c = 0" unfolding config_time_def by simp
+
+
+lemma final_steps_config_time[dest]: "is_final (steps n c) \<Longrightarrow> steps n c = steps (config_time c) c" by simp
+
+lemma conf_time_steps_finalI: "\<exists>n. is_final (steps n c) \<and> P (steps n c) \<Longrightarrow>
+  is_final (steps (config_time c) c) \<and> P (steps (config_time c) c)" by force
+
+lemma conf_time_steps_final_iff:
+  "(\<exists>n. is_final (steps n c) \<and> P (steps n c)) \<longleftrightarrow>
+  (is_final (steps (config_time c) c) \<and> P (steps (config_time c) c))"
+  by (intro iffI conf_time_steps_finalI) blast+
+
+
+definition "time w \<equiv> config_time (initial_config w)"
+declare (in -) TM.time_def[simp]
+
+lemma time_altdef: "time w = (LEAST n. is_final (run n w))"
+  unfolding TM.run_def using config_time_def by simp
+
+lemma time_leI[intro]:
+  "is_final (run n w) \<Longrightarrow> time w \<le> n"
+  unfolding run_def time_def by (rule conf_time_geI)
+
+lemma run_time_halts[dest]: "halts w \<Longrightarrow> is_final (run (time w) w)" by auto
+
+lemma config_time_offset:
+  fixes c0
+  defines "n \<equiv> config_time c0"
+  assumes "halts_config c0"
+  shows "config_time (steps n1 c0) = n - n1"
+proof (cases "is_final (steps n1 c0)")
+  assume f: "is_final (steps n1 c0)"
+  then have "n1 \<ge> n" unfolding n_def by blast
+  with f show ?thesis unfolding n_def by simp
+next
+  assume nf: "\<not> is_final (steps n1 c0)"
+
+  let ?N = "{n2. is_final (steps n2 (steps n1 c0))}"
+
+  have "{n. is_final (steps n c0)} = {n. \<exists>n2. n = n1 + n2 \<and> is_final (steps n2 (steps n1 c0))}"
+    (is "{n. ?lhs n} = {n. ?rhs n}")
+  proof (rule sym, intro Collect_eqI iffI)
+    fix n assume "?lhs n"
+    with nf have "n > n1" by blast
+    then have "\<exists>n2. n = n1 + n2" by (intro le_Suc_ex less_imp_le_nat)
+    then obtain n2 where "n = n1 + n2" ..
+    from \<open>?lhs n\<close> have "is_final (steps n2 (steps n1 c0))" unfolding \<open>n = n1 + n2\<close> by simp
+    with \<open>n = n1 + n2\<close> show "?rhs n" by blast
+  next
+    fix n assume "?rhs n"
+    then obtain n2 where "n = n1 + n2" and "is_final (steps n2 (steps n1 c0))" by blast
+    then show "?lhs n" by simp
+  qed
+  then have *: "{n. is_final (steps n c0)} = (\<lambda>n2. n1 + n2) ` ?N" unfolding image_Collect .
+
+  have "n = (LEAST n. is_final (steps n c0))" unfolding n_def config_time_def ..
+  also have "... = (LEAST n. n \<in> {n. is_final (steps n c0)})" by simp
+  also have "... = n1 + (LEAST n. is_final (steps n (steps n1 c0)))" unfolding *
+  proof (subst Least_mono, unfold mem_Collect_eq)
+    show "mono (\<lambda>n2. n1 + n2)" by (intro monoI add_left_mono)
+
+    let ?n = "config_time c0" let ?n2 = "?n - n1"
+    have *: "x \<in> ?N \<longleftrightarrow> x \<ge> ?n2" for x
+      unfolding mem_Collect_eq steps_plus le_diff_conv add.commute[of x n1]
+      using \<open>halts_config c0\<close> by (fact conf_time_ge_iff)
+    then show "\<exists>n\<in>?N. \<forall>n'\<in>?N. n \<le> n'" by blast
+  qed blast
+  also have "... = n1 + config_time (steps n1 c0)" unfolding config_time_def ..
+  finally show ?thesis by presburger
+qed
+
+
+lemma config_time_eqI[intro]:
+  assumes "TM.halts_config M1 c1"
+    and "\<And>n. TM.is_final M1 (TM.steps M1 (n1 + n) c1) \<longleftrightarrow> TM.is_final M2 (TM.steps M2 n c2)"
+  shows "TM.config_time M1 c1 - n1 = TM.config_time M2 c2"
+proof -
+  from \<open>TM.halts_config M1 c1\<close> have "TM.config_time M1 c1 - n1 = TM.config_time M1 (TM.steps M1 n1 c1)"
+    by (subst TM.config_time_offset) auto
+  also have "... = TM.config_time M2 c2" unfolding TM.config_time_def TM.steps_plus unfolding assms ..
+  finally show ?thesis .
+qed
+
+lemma time_eqI[intro]:
+  assumes "TM.halts M1 w1"
+    and "\<And>n. TM.is_final M1 (TM.run M1 (n1 + n) w1) \<longleftrightarrow> TM.is_final M2 (TM.run M2 n w2)"
+  shows "TM.time M1 w1 - n1 = TM.time M2 w2"
+  using assms unfolding TM.time_def TM.run_def TM.halts_def by (fact config_time_eqI)
+
+
+lemma (in Rej_TM) rej_tm_time: "time w = 0" by simp
+
+end \<comment> \<open>context \<^locale>\<open>TM\<close>\<close>
+
+
+subsubsection\<open>Time Function Wrapper\<close>
+
+text\<open>From @{cite \<open>ch.~12.1\<close> hopcroftAutomata1979}:
   ``[...] it is reasonable to assume that any time complexity function \<open>T(n)\<close> is
     at least \<open>n + 1\<close>, for this is the time needed just to read the input and verify that the
     end has been reached by reading the first blank.* We thus make the convention
@@ -79,6 +216,10 @@ proof -
 qed
 
 
+subsubsection\<open>Time-Bounded Execution\<close>
+
+text\<open>Predicates to verify that TMs halt within a given time-bound.\<close>
+
 context TM begin
 
 definition time_bounded_word :: "('c::semiring_1 \<Rightarrow> 'd::floor_ceiling) \<Rightarrow> 's list \<Rightarrow> bool"
@@ -135,9 +276,8 @@ lemma time_bounded_mono:
   shows "time_bounded T"
   by (rule time_bounded_mono', rule tcomp_mono) fact+
 
-lemma time_bounded_altdef2:
-  "time_bounded T \<longleftrightarrow> (\<forall>w. halts w \<and> time w \<le> tcomp\<^sub>w T w)"
-  unfolding time_bounded_def by (intro iff_allI) blast
+lemma time_bounded_altdef2: "time_bounded T \<longleftrightarrow> (\<forall>w. halts w \<and> time w \<le> tcomp\<^sub>w T w)"
+  unfolding time_bounded_def by blast
 
 corollary time_bounded_time: "time_bounded T \<Longrightarrow> time w \<le> tcomp\<^sub>w T w"
   unfolding time_bounded_altdef2 by blast
